Ed: Work towards barrett reduction

code/experimental/ed25519/Hacl.Impl.BignumQ.Mul.fst
@@ -7,20 +7,31 @@ open FStar.Mul
 open Lib.IntTypes
 open Lib.Buffer
 
+module SE = Spec.Ed25519
+
+module S56 = Hacl.Spec.Ed25519.Field56.Definition
+
 #reset-options "--z3rlimit 20 --max_fuel 0 --max_ifuel 0"
 
+noextract
+let mu_v : n:nat = 0xfffffffffffffffffffffffffffffffeb2106215d086329a7ed9ce5a30a2c131b
+
 inline_for_extraction noextract
-val make_m:
+val make_q:
   m:qelemB ->
   Stack unit
     (requires fun h -> live h m)
-    (ensures  fun h0 _ h1 -> modifies (loc m) h0 h1)
-let make_m m =
+    (ensures  fun h0 _ h1 -> modifies (loc m) h0 h1 /\
+      F56.as_nat h1 m == SE.q
+    )
+let make_q m =
   m.(0ul) <- u64 0x12631a5cf5d3ed;
   m.(1ul) <- u64 0xf9dea2f79cd658;
   m.(2ul) <- u64 0x000000000014de;
   m.(3ul) <- u64 0x00000000000000;
-  m.(4ul) <- u64 0x00000010000000
+  m.(4ul) <- u64 0x00000010000000;
+  assert_norm (S56.as_nat5 (u64 0x12631a5cf5d3ed, u64 0xf9dea2f79cd658,
+    u64 0x000000000014de, u64 0x00000000000000,  u64 0x00000010000000) == SE.q)
 
 inline_for_extraction noextract
 val make_mu:
@@ -43,7 +54,10 @@ val choose:
   -> b:uint64{v b == 0 \/ v b == 1} ->
   Stack unit
     (requires fun h -> live h x /\ live h y /\ live h z)
-    (ensures  fun h0 _ h1 -> modifies (loc z) h0 h1)
+    (ensures  fun h0 _ h1 -> modifies (loc z) h0 h1 /\
+      (v b == 0 ==> Seq.equal (as_seq h1 z) (as_seq h0 y)) /\
+      (v b == 1 ==> Seq.equal (as_seq h1 z) (as_seq h0 x))
+    )
 let choose z x y b =
   let mask = b -. u64 1 in
   let x0 = x.(0ul) in
@@ -56,35 +70,67 @@ let choose z x y b =
   let y2 = y.(2ul) in
   let y3 = y.(3ul) in
   let y4 = y.(4ul) in
-  let z0 = ((y0 ^. x0) &. mask) ^. x0 in
-  let z1 = ((y1 ^. x1) &. mask) ^. x1 in
-  let z2 = ((y2 ^. x2) &. mask) ^. x2 in
-  let z3 = ((y3 ^. x3) &. mask) ^. x3 in
-  let z4 = ((y4 ^. x4) &. mask) ^. x4 in
-  Hacl.Bignum25519.make_u64_5 z z0 z1 z2 z3 z4
+  let z0 = x0 ^. ((y0 ^. x0) &. mask) in
+  let z1 = x1 ^. ((y1 ^. x1) &. mask) in
+  let z2 = x2 ^. ((y2 ^. x2) &. mask) in
+  let z3 = x3 ^. ((y3 ^. x3) &. mask) in
+  let z4 = x4 ^. ((y4 ^. x4) &. mask) in
+  Hacl.Bignum25519.make_u64_5 z z0 z1 z2 z3 z4;
+  let lemma_mask0 () : Lemma
+    (requires v b == 0)
+    (ensures y0 == z0 /\ y1 == z1 /\ y2 == z2 /\ y3 == z3 /\ y4 == z4)
+    =
+    Lib.IntTypes.Compatibility.uintv_extensionality mask (ones U64 SEC);
+    logand_ones (y0 ^. x0);
+    logand_ones (y1 ^. x1);
+    logand_ones (y2 ^. x2);
+    logand_ones (y3 ^. x3);
+    logand_ones (y4 ^. x4);
+    logxor_lemma x0 y0;
+    logxor_lemma x1 y1;
+    logxor_lemma x2 y2;
+    logxor_lemma x3 y3;
+    logxor_lemma x4 y4
+  in
+  let lemma_mask1 () : Lemma
+    (requires v b == 1)
+    (ensures x0 == z0 /\ x1 == z1 /\ x2 == z2 /\ x3 == z3 /\ x4 == z4)
+    =
+    assert (v mask == 0);
+    logand_zeros (y0 ^. x0);
+    logand_zeros (y1 ^. x1);
+    logand_zeros (y2 ^. x2);
+    logand_zeros (y3 ^. x3);
+    logand_zeros (y4 ^. x4);
+    logxor_lemma x0 x0;
+    logxor_lemma x1 x0;
+    logxor_lemma x2 x0;
+    logxor_lemma x3 x0;
+    logxor_lemma x4 x0
+  in
+  Classical.move_requires lemma_mask1 ();
+  Classical.move_requires lemma_mask0 ()
 
 inline_for_extraction noextract
-let lt (a:uint64) (b:uint64) : uint64 = (a -. b) >>. 63ul
+let lt (a:uint64{v a < pow2 63}) (b:uint64{v b < pow2 63}) : (c:uint64{if v a >= v b then v c == 0 else v c == 1})
+  = (a -. b) >>. 63ul
 
 inline_for_extraction noextract
-let shiftl_56 (b:uint64) : uint64 = b <<. 56ul
+let shiftl_56 (b:uint64{v b == 0 \/ v b == 1}) : (c:uint64{v c == 0x100000000000000 * v b})
+  =
+    assert_norm ((1 * pow2 56) % pow2 64 == 0x100000000000000);
+    assert_norm ((0 * pow2 56) % pow2 64 == 0);
+    b <<. 56ul
 
 inline_for_extraction noextract
-val subm_step: x:uint64 -> y:uint64 -> uint64 & uint64
-let subm_step x y =
-  let b  = lt x y in
-  let t = (shiftl_56 b +. x) -. y in
-  b, t
+let shiftl_40 (b:uint64{v b == 0 \/ v b == 1}) : (c:uint64{v c == 0x10000000000 * v b}) =
+  assert_norm ((1 * pow2 40) % pow2 64 == 0x10000000000);
+  assert_norm ((0 * pow2 40) % pow2 64 == 0);
+  b <<. 40ul
 
-inline_for_extraction noextract
-let shiftl_40 (b:uint64) : uint64 = b <<. 40ul
-
-inline_for_extraction noextract
-val subm_last_step: x:uint64 -> y:uint64 -> uint64 & uint64
-let subm_last_step x y =
-  let b  = lt x y in
-  let t = (shiftl_40 b +. x) -. y in
-  b, t
+let lemma_mult_distr4 (n:nat) (a b c d:nat) : Lemma
+  (n * (a - b - c + d) == n * a - n * b - n * c + n * d)
+  = ()
 
 inline_for_extraction noextract
 val sub_mod_264:
@@ -92,9 +138,48 @@ val sub_mod_264:
   -> x:qelemB
   -> y:qelemB ->
   Stack unit
-    (requires fun h -> live h x /\ live h y /\ live h z)
-    (ensures fun h0 _ h1 -> modifies (loc z) h0 h1)
+    (requires fun h -> live h x /\ live h y /\ live h z /\
+      F56.as_nat h x < pow2 264 /\
+      F56.as_nat h y < pow2 264 /\
+      (let s = as_seq h x in
+       let op_String_Access = Seq.index in
+       v s.[0] < 0x100000000000000 /\
+       v s.[1] < 0x100000000000000 /\
+       v s.[2] < 0x100000000000000 /\
+       v s.[3] < 0x100000000000000 /\
+       v s.[4] < 0x100000000000000) /\
+      (let s = as_seq h y in
+       let op_String_Access = Seq.index in
+       v s.[0] < 0x100000000000000 /\
+       v s.[1] < 0x100000000000000 /\
+       v s.[2] < 0x100000000000000 /\
+       v s.[3] < 0x100000000000000 /\
+       v s.[4] < 0x100000000000000)
+    )
+    (ensures fun h0 _ h1 -> modifies (loc z) h0 h1 /\
+      // (let s = as_seq h1 z in
+      //  let op_String_Access = Seq.index in
+      //  v s.[0] < 0x100000000000000 /\
+      //  v s.[1] < 0x100000000000000 /\
+      //  v s.[2] < 0x100000000000000 /\
+      //  v s.[3] < 0x100000000000000 /\
+      //  v s.[4] < 0x100000000000000) /\
+      (F56.as_nat h0 x < F56.as_nat h0 y ==>
+        F56.as_nat h1 z == pow2 264 + F56.as_nat h0 x - F56.as_nat h0 y) /\
+      (F56.as_nat h0 x >= F56.as_nat h0 y ==>
+        F56.as_nat h1 z ==  F56.as_nat h0 x - F56.as_nat h0 y)
+    )
+
+#push-options "--z3rlimit 600"
+
 let sub_mod_264 z x y =
+  assert_norm(pow2 264 = 0x1000000000000000000000000000000000000000000000000000000000000000000);
+  assert_norm(pow2 64 = 0x10000000000000000);
+  assert_norm(pow2 56 = 0x100000000000000);
+  assert_norm(pow2 40 = 0x10000000000);
+  assert_norm(pow2 32 = 0x100000000);
+  let h0 = get() in
+
   let x0 = x.(0ul) in
   let x1 = x.(1ul) in
   let x2 = x.(2ul) in
@@ -106,30 +191,160 @@ let sub_mod_264 z x y =
   let y3 = y.(3ul) in
   let y4 = y.(4ul) in
   let pb = y0 in
-  let b  = lt x0 y0 in
-  let t0 = (shiftl_56 b +. x0) -. y0 in
-  let y1 = y1 +. b in
-  let b  = lt x1 y1 in
-  let t1 = (shiftl_56 b +. x1) -. y1 in
-  let y2 = y2 +. b in
-  let b  = lt x2 y2 in
-  let t2 = (shiftl_56 b +. x2) -. y2 in
-  let y3 = y3 +. b in
-  let b  = lt x3 y3 in
-  let t3 = (shiftl_56 b +. x3) -. y3 in
-  let y4 = y4 +. b in
-  let b  = lt x4 y4 in
-  let t4 = (shiftl_40 b +. x4) -. y4 in
+  let b0  = lt x0 y0 in
+  let t0 = (shiftl_56 b0 +. x0) -. y0 in
+  let y1' = y1 +. b0 in
+  let b1  = lt x1 y1' in
+  let t1 = (shiftl_56 b1 +. x1) -. y1' in
+  let y2' = y2 +. b1 in
+  let b2  = lt x2 y2' in
+  let t2 = (shiftl_56 b2 +. x2) -. y2' in
+  let y3' = y3 +. b2 in
+  let b3  = lt x3 y3' in
+  let t3 = (shiftl_56 b3 +. x3) -. y3' in
+  let y4' = y4 +. b3 in
+  let b4  = lt x4 y4' in
+  let t4 = (shiftl_40 b4 +. x4) -. y4' in
+
+  calc (==) {
+    v t0 <: int;
+    (==) { Math.Lemmas.small_mod (v (shiftl_56 b0) + v x0) (pow2 64);
+           Math.Lemmas.small_mod (v (shiftl_56 b0 +. x0) - v y0) (pow2 64) }
+    v x0 - v y0 + 0x100000000000000 * v b0;
+  };
+  calc (==) {
+    v t1 <: int;
+    (==) {  Math.Lemmas.small_mod (v y1 + v b0) (pow2 64);
+            Math.Lemmas.small_mod (v (shiftl_56 b1) + v x1) (pow2 64);
+            Math.Lemmas.small_mod (v (shiftl_56 b1 +. x1) - v y1') (pow2 64) }
+     v x1 - v y1 - v b0 + 0x100000000000000 * v b1;
+  };
+  calc (==) {
+    v t2 <: int;
+    (==) {  Math.Lemmas.small_mod (v y2 + v b1) (pow2 64);
+            Math.Lemmas.small_mod (v (shiftl_56 b2) + v x2) (pow2 64);
+            Math.Lemmas.small_mod (v (shiftl_56 b2 +. x2) - v y2') (pow2 64) }
+     v x2 - v y2 - v b1 + 0x100000000000000 * v b2;
+  };
+  calc (==) {
+    v t3 <: int;
+    (==) {  Math.Lemmas.small_mod (v y3 + v b2) (pow2 64);
+            Math.Lemmas.small_mod (v (shiftl_56 b3) + v x3) (pow2 64);
+            Math.Lemmas.small_mod (v (shiftl_56 b3 +. x3) - v y3') (pow2 64) }
+     v x3 - v y3 - v b2 + 0x100000000000000 * v b3;
+  };
+  // calc (==) {
+  //   v t4 <: int;
+  //   (==) {  Math.Lemmas.small_mod (v y4 + v b3) (pow2 64);
+  //           assert_norm (pow2 40 + pow2 56 < pow2 64);
+  //           Math.Lemmas.small_mod (v (shiftl_40 b4) + v x4) (pow2 64) }
+  //    (( 0x100000000000000 * v b4 + v x4) - (v y4 + v b3)) % pow2 64;
+  // };
+  admit();
+
+  admit();
+  // assert_norm (0x100000000000000 + (0x100000000000000 - 1) * pow2 56 + (0x100000000000000 - 1) * pow2 112 + (0x100000000000000 - 1) * pow2 168 + (0x10000000000 - 1) * pow2 224 == pow2 264);
+  // Math.Lemmas.small_mod (v y1 + v b0) (pow2 64);
+  // Math.Lemmas.small_mod (v ((shiftl_56 b1 +. x1) -. y1')) (pow2 64);
+  // Math.Lemmas.small_mod (v (shiftl_56 b1 +. x1)) (pow2 64);
+  // assert (v t1 == v x1 - v y1 - v b0 + 0x100000000000000 * v b1);
+  // // assert (v t1 < 0x10000000000);
+  // // admit();
+  // // assume (v x1 - v y1' + 0x100000000000000 * v b1 == v t1 /\ v t1 < 0x10000000000);
+  // Math.Lemmas.small_mod (v y2 + v b1) (pow2 64);
+  // Math.Lemmas.small_mod (v ((shiftl_56 b2 +. x2) -. y2')) (pow2 64);
+  // Math.Lemmas.small_mod (v (shiftl_56 b2 +. x2)) (pow2 64);
+  // admit();
+  // assert (v t2 == v x2 - v y2 - v b1 + 0x100000000000000 * v b2);
+  // admit();
+  // Math.Lemmas.small_mod (v y3 + v b2) (pow2 64);
+  // assume (v t3 == v x3 - v y3 - v b2 + 0x100000000000000 * v b3);
+  // Math.Lemmas.small_mod (v y4 + v b3) (pow2 64);
+  // assume (v t4 == v x4 - v y4 - v b3 - 0x10000000000 * v b4);
+  // let lemma_b () : Lemma
+  //   (requires b4 == 0)
+  //   (ensures F56.as_nat h0 x < F56.as_nat h0 y)
+  //   = admit()
+  // in
+  // calc (==) {
+  //   0x100000000000000 * v b0  + v x0 - v y0 +
+  //   0x100000000000000 * (v x1 - v y1 - v b0 + 0x100000000000000 * v b1) +
+  //   0x10000000000000000000000000000 * (v x2 - v y2 - v b1 + 0x100000000000000 * v b2) +
+  //   0x1000000000000000000000000000000000000000000 * (v x3 - v y3 - v b2 + 0x100000000000000 * v b3) +
+  //   0x100000000000000000000000000000000000000000000000000000000 * (
+  //     v x4 - v y4 - v b3 + 0x10000000000 * v b4);
+  //   (==) {lemma_mult_distr4 0x100000000000000 (v x1) (v y1) (v b0) (0x100000000000000 * v b1);
+  //         lemma_mult_distr4 0x10000000000000000000000000000 (v x2) (v y2) (v b1) (0x100000000000000 * v b2);
+  //         lemma_mult_distr4 0x1000000000000000000000000000000000000000000 (v x3) (v y3) (v b2) (0x100000000000000 * v b3);
+  //         lemma_mult_distr4 0x100000000000000000000000000000000000000000000000000000000 (v x4) (v y4) (v b3) (0x100000000000000 * v b4)
+  //   }
+  //    v x0 - v y0 +
+  //   0x100000000000000 * v x1 - 0x100000000000000 * v y1 +
+  //   0x100000000000000 * (0x100000000000000 * v b1) +
+  //   0x10000000000000000000000000000 * v x2 -
+  //   0x10000000000000000000000000000 * v y2 -
+  //   0x10000000000000000000000000000 * v b1 +
+  //   0x10000000000000000000000000000 * (0x100000000000000 * v b2) +
+  //   0x1000000000000000000000000000000000000000000 * v x3 -
+  //   0x1000000000000000000000000000000000000000000 * v y3 -
+  //   0x1000000000000000000000000000000000000000000 * v b2 +
+  //   0x1000000000000000000000000000000000000000000 * (0x100000000000000 * v b3) +
+  //   0x100000000000000000000000000000000000000000000000000000000 * v x4 -
+  //   0x100000000000000000000000000000000000000000000000000000000 * v y4 -
+  //   0x100000000000000000000000000000000000000000000000000000000 * v b3 +
+  //   0x100000000000000000000000000000000000000000000000000000000 * (0x10000000000 * v b4);
+  //   (==) { Math.Lemmas.paren_mul_right 0x100000000000000 0x100000000000000 (v b1);
+  //          Math.Lemmas.paren_mul_right 0x10000000000000000000000000000 0x100000000000000 (v b2);
+  //          Math.Lemmas.paren_mul_right 0x1000000000000000000000000000000000000000000  0x100000000000000 (v b3);
+  //          Math.Lemmas.paren_mul_right 0x100000000000000000000000000000000000000000000000000000000 0x100000000000000 (v b4);
+  //          assert_norm (0x100000000000000 * 0x100000000000000 == 0x10000000000000000000000000000)
+  //   }
+
+  //    v x0 - v y0 +
+  //   0x100000000000000 * v x1 - 0x100000000000000 * v y1 +
+  //   0x10000000000000000000000000000 * v x2 -
+  //   0x10000000000000000000000000000 * v y2 +
+  //   0x1000000000000000000000000000000000000000000 * v x3 -
+  //   0x1000000000000000000000000000000000000000000 * v y3 +
+  //   0x100000000000000000000000000000000000000000000000000000000 * v x4 -
+  //   0x100000000000000000000000000000000000000000000000000000000 * v y4 +
+  //   pow2 264 * v b4;
+  //   (==) { }
+  //   S56.as_nat5 (x0, x1, x2, x3, x4) - S56.as_nat5 (y0, y1, y2, y3, y4) + pow2 264 * v b4;
+  // };
+  // assume (v b4 <> 0 <==> F56.as_nat h0 x < F56.as_nat h0 y);
   Hacl.Bignum25519.make_u64_5 z t0 t1 t2 t3 t4
+
+#pop-options
 
 inline_for_extraction noextract
 val subm_conditional:
     z:qelemB
   -> x:qelemB ->
   Stack unit
-    (requires fun h -> live h x /\ live h z /\ disjoint x z)
-    (ensures  fun h0 _ h1 -> modifies (loc z) h0 h1)
+    (requires fun h -> live h x /\ live h z /\ disjoint x z /\
+      (let s = as_seq h x in
+       let op_String_Access = Seq.index in
+       v s.[0] < 0x100000000000000 /\
+       v s.[1] < 0x100000000000000 /\
+       v s.[2] < 0x100000000000000 /\
+       v s.[3] < 0x100000000000000 /\
+       v s.[4] < 0x100000000000000)
+    )
+    (ensures  fun h0 _ h1 -> modifies (loc z) h0 h1 /\
+      (let s = as_seq h1 z in
+       let op_String_Access = Seq.index in
+       v s.[0] < 0x100000000000000 /\
+       v s.[1] < 0x100000000000000 /\
+       v s.[2] < 0x100000000000000 /\
+       v s.[3] < 0x100000000000000 /\
+       v s.[4] < 0x100000000000000) /\
+     (F56.as_nat h0 x >= SE.q ==> F56.as_nat h1 z == F56.as_nat h0 x - SE.q) /\
+     (F56.as_nat h0 x < SE.q ==> F56.as_nat h1 z == F56.as_nat h0 x)
+    )
+
 let subm_conditional z x =
+  admit();
   let h' = ST.get () in
   push_frame();
   let tmp = create 5ul (u64 0) in
@@ -165,16 +380,11 @@ let subm_conditional z x =
   pop_frame()
 
 inline_for_extraction noextract
-val split_56: x:uint128 -> uint128 & uint64
-let split_56 x =
-  let carry = x >>. 56ul in
-  let t     = to_u64 x &. u64 0xffffffffffffff in
-  carry, t
-
-inline_for_extraction noextract
-val mod_40: x:uint128 -> uint64
+val mod_40: x:uint128 -> (c:uint64{v c == v x % pow2 40})
 let mod_40 x =
   let x' = to_u64 x in
+  assert_norm (pow2 40 - 1  == 0xffffffffff);
+  logand_mask x' (u64 0xffffffffff) 40;
   let x'' = x' &. u64 0xffffffffff in
   x''
 
@@ -184,8 +394,33 @@ val low_mul_5:
   -> x:qelemB
   -> y:qelemB ->
   Stack unit
-    (requires fun h -> live h z /\ live h x /\ live h y)
-    (ensures  fun h0 _ h1 -> modifies (loc z) h0 h1)
+    (requires fun h -> live h z /\ live h x /\ live h y /\
+      (let s = as_seq h x in
+       let op_String_Access = Seq.index in
+       v s.[0] < 0x100000000000000 /\
+       v s.[1] < 0x100000000000000 /\
+       v s.[2] < 0x100000000000000 /\
+       v s.[3] < 0x100000000000000 /\
+       v s.[4] < 0x100000000000000) /\
+      (let s = as_seq h y in
+       let op_String_Access = Seq.index in
+       v s.[0] < 0x100000000000000 /\
+       v s.[1] < 0x100000000000000 /\
+       v s.[2] < 0x100000000000000 /\
+       v s.[3] < 0x100000000000000 /\
+       v s.[4] < 0x100000000000000)
+    )
+    (ensures  fun h0 _ h1 -> modifies (loc z) h0 h1 /\
+      (let s = as_seq h1 z in
+       let op_String_Access = Seq.index in
+       v s.[0] < 0x100000000000000 /\
+       v s.[1] < 0x100000000000000 /\
+       v s.[2] < 0x100000000000000 /\
+       v s.[3] < 0x100000000000000 /\
+       v s.[4] < 0x100000000000000) /\
+     F56.as_nat h1 z == (F56.as_nat h0 x * F56.as_nat h0 y) % pow2 264
+    )
+
 let low_mul_5 z x y =
   let x0 = x.(0ul) in
   let x1 = x.(1ul) in
@@ -214,6 +449,7 @@ let low_mul_5 z x y =
   let xy40 = mul64_wide x4 y0 in
   let x    = xy00 in
   let carry = x >>. 56ul in
+  assert_norm (0xffffffffffffff == pow2 56 - 1);
   let t     = to_u64 x &. u64 0xffffffffffffff in
   let t0  = t in
   let x = xy01 +. xy10 +. carry in
@@ -229,6 +465,7 @@ let low_mul_5 z x y =
   let t     = to_u64 x &. u64 0xffffffffffffff in
   let t3 = t in
   let t4 = mod_40 (xy04 +. xy13 +. xy22 +. xy31 +. xy40 +. carry) in
+  admit();
   Hacl.Bignum25519.make_u64_5 z t0 t1 t2 t3 t4
 
 inline_for_extraction noextract
@@ -237,9 +474,39 @@ val mul_5:
   -> x:qelemB
   -> y:qelemB ->
   Stack unit
-    (requires fun h -> live h z /\ live h x /\ live h y)
-    (ensures fun h0 _ h1 -> modifies (loc z) h0 h1)
+    (requires fun h -> live h z /\ live h x /\ live h y /\
+      (let s = as_seq h x in
+       let op_String_Access = Seq.index in
+       v s.[0] < 0x100000000000000 /\
+       v s.[1] < 0x100000000000000 /\
+       v s.[2] < 0x100000000000000 /\
+       v s.[3] < 0x100000000000000 /\
+       v s.[4] < 0x100000000000000) /\
+      (let s = as_seq h y in
+       let op_String_Access = Seq.index in
+       v s.[0] < 0x100000000000000 /\
+       v s.[1] < 0x100000000000000 /\
+       v s.[2] < 0x100000000000000 /\
+       v s.[3] < 0x100000000000000 /\
+       v s.[4] < 0x100000000000000)
+    )
+    (ensures fun h0 _ h1 -> modifies (loc z) h0 h1 /\
+      F56.feval_wide9 h1 z == F56.as_nat h0 x * F56.as_nat h0 y /\
+      (let s = as_seq h1 z in
+       let op_String_Access = Seq.index in
+       v s.[0] < 0x10000000000000000000000000000 /\
+       v s.[1] < 0x20000000000000000000000000000 /\
+       v s.[2] < 0x30000000000000000000000000000 /\
+       v s.[3] < 0x40000000000000000000000000000 /\
+       v s.[4] < 0x50000000000000000000000000000 /\
+       v s.[5] < 0x40000000000000000000000000000 /\
+       v s.[6] < 0x30000000000000000000000000000 /\
+       v s.[7] < 0x20000000000000000000000000000 /\
+       v s.[8] < 0x10000000000000000000000000000)
+    )
+
 let mul_5 z x y =
+  admit();
   let x0 = x.(0ul) in
   let x1 = x.(1ul) in
   let x2 = x.(2ul) in
@@ -300,8 +567,12 @@ val carry:
   -> z:lbuffer uint128 9ul ->
   Stack unit
     (requires fun h -> live h z /\ live h t)
-    (ensures  fun h0 _ h1 -> modifies (loc t) h0 h1)
+    (ensures  fun h0 _ h1 -> modifies (loc t) h0 h1 /\
+      fits_elem10 (as_seq h1 t) /\
+      F56.as_nat10 h1 t == F56.feval_wide9 h0 z
+    )
 let carry out z =
+  admit();
   let z0 = z.(0ul) in
   let z1 = z.(1ul) in
   let z2 = z.(2ul) in
@@ -365,8 +636,11 @@ val mod_264:
   -> t:lbuffer uint64 10ul ->
   Stack unit
     (requires fun h -> live h r /\ live h t)
-    (ensures  fun h0 _ h1 ->  modifies (loc r) h0 h1)
+    (ensures  fun h0 _ h1 ->  modifies (loc r) h0 h1 /\
+      F56.as_nat h1 r == F56.as_nat10 h0 t % pow2 264
+    )
 let mod_264 r t =
+  admit();
   let x0 = t.(0ul) in
   let x1 = t.(1ul) in
   let x2 = t.(2ul) in
@@ -397,8 +671,11 @@ val div_248:
   -> t:lbuffer uint64 10ul ->
   Stack unit
     (requires fun h -> live h q /\ live h t)
-    (ensures  fun h0 _ h1 -> modifies (loc q) h0 h1)
+    (ensures  fun h0 _ h1 -> modifies (loc q) h0 h1 /\
+      F56.as_nat h1 q == F56.as_nat10 h0 t / pow2 248
+    )
 let div_248 out t =
+  admit();
   let x0 = t.(0ul) in
   let x1 = t.(1ul) in
   let x2 = t.(2ul) in
@@ -422,8 +699,11 @@ val div_264:
   -> t:lbuffer uint64 10ul ->
   Stack unit
     (requires fun h -> live h q /\ live h t)
-    (ensures  fun h0 _ h1 -> modifies (loc q) h0 h1)
+    (ensures  fun h0 _ h1 -> modifies (loc q) h0 h1 /\
+      F56.as_nat h1 q == F56.as_nat10 h0 t / pow2 264
+    )
 let div_264 out t =
+  admit();
   let x0 = t.(0ul) in
   let x1 = t.(1ul) in
   let x2 = t.(2ul) in
@@ -451,11 +731,17 @@ val barrett_reduction__1:
     (requires fun h ->
       live h t /\ live h qmu /\ live h mu /\ live h tmp /\
       disjoint tmp mu /\ disjoint tmp qmu)
-    (ensures fun h0 _ h1 ->  modifies (loc qmu |+| loc tmp) h0 h1)
+    (ensures fun h0 _ h1 ->  modifies (loc qmu |+| loc tmp) h0 h1 /\
+      (let q = F56.as_nat10 h0 t / pow2 248 in
+       let qmu = q * mu_v in
+       let qmu264 = qmu / pow2 264 in
+       F56.as_nat h1 (gsub tmp 20ul 5ul) == qmu264)
+    )
 let barrett_reduction__1 qmu t mu tmp =
   let q   = sub tmp 0ul 5ul in
   let qmu'  = sub tmp 10ul 10ul in
   let qmu_264 = sub tmp 20ul 5ul in
+  admit();
   div_248 q t;
   mul_5 qmu q mu;
   carry qmu' qmu;
@@ -471,11 +757,13 @@ val barrett_reduction__2:
       live h t /\ live h m /\ live h tmp /\
       disjoint tmp m /\ disjoint tmp t)
     (ensures fun h0 _ h1 -> modifies (loc tmp) h0 h1)
+
 let barrett_reduction__2 t m tmp =
   let qmul = sub tmp 0ul 5ul in
   let r    = sub tmp 5ul 5ul in
   let qmu_264 = sub tmp 20ul 5ul in
   let s    = sub tmp 25ul 5ul in
+  admit();
   mod_264 r t;
   low_mul_5 qmul qmu_264 m;
   sub_mod_264 s r qmul
@@ -494,6 +782,7 @@ val barrett_reduction__:
     (ensures fun h0 _ h1 -> modifies (loc z |+| loc tmp) h0 h1)
 let barrett_reduction__ z t m mu tmp =
   let s   = sub tmp 25ul 5ul in
+  admit();
   push_frame();
   let qmu = create 9ul (u128 0) in
   let h0 = ST.get () in
@@ -523,15 +812,16 @@ let barrett_reduction_ z t =
   let m   = sub tmp 0ul 5ul in
   let mu  = sub tmp 5ul 5ul in
   let tmp = sub tmp 10ul 30ul in
-  make_m m;
+  make_q m;
   make_mu mu;
   barrett_reduction__ z t m mu tmp;
   pop_frame()
 
 let barrett_reduction z t =
+  admit();
   barrett_reduction_ z t
 
-#reset-options "--max_fuel 0"
+#reset-options "--z3rlimit 40 --max_fuel 0 --max_ifuel 0"
 
 let mul_modq out x y =
   push_frame();
@@ -539,8 +829,7 @@ let mul_modq out x y =
   let z  = create 9ul (u128 0) in
   mul_5 z x y;
   carry z' z;
-  barrett_reduction_ out z';
-  admit();
+  barrett_reduction out z';
   pop_frame()
 
 inline_for_extraction noextract
